generational/spec/GC.Gen.PromoteUpdate.Positional.fsti
@@ -1,0 +1,90 @@
+module GC.Gen.PromoteUpdate.Positional
+
+open FStar.Seq
+module U64 = FStar.UInt64
+module U8 = FStar.UInt8
+
+open GC.Spec.Base
+open GC.Spec.Heap
+open GC.Spec.Object
+open GC.Spec.Fields
+open GC.Gen.Base
+open GC.Gen.MinorHeap
+open GC.Gen.Reachability
+open GC.Gen.Remembered
+open GC.Gen.Promote
+open GC.Gen.WriteBodyLemmas
+
+module AllocLemmas = GC.Spec.Allocator.Lemmas
+
+val update_all_objects_positional_step
+  (major: heap) (fwd: forwarding_map) (pos: hp_addr)
+  : Lemma (requires well_formed_heap_part1 major /\
+                    heap_objects_dense major /\
+                    U64.v pos + 8 < heap_size /\
+                    Seq.mem (f_address pos) (objects zero_addr major) /\
+                    Seq.length (objects pos major) > 0 /\
+                    is_blue (f_address pos) major = false)
+          (ensures (let hdr = read_word major pos in
+                    let wz = U64.v (getWosize hdr) in
+                    let obj : obj_addr = f_address pos in
+                    let major' = update_object_pointers major obj wz fwd 0 in
+                    let next_nat = U64.v pos + (wz + 1) * 8 in
+                    next_nat <= heap_size /\ next_nat % 8 == 0 /\ next_nat < pow2 64 /\
+                    U64.v obj + wz * 8 <= heap_size /\
+                    well_formed_heap_part1 major' /\
+                    heap_objects_dense major' /\
+                    objects zero_addr major' == objects zero_addr major /\
+                    (next_nat < heap_size ==>
+                      update_all_objects_aux major' (objects (U64.uint_to_t next_nat) major') fwd 0 ==
+                        update_all_objects_aux major (objects pos major) fwd 0) /\
+                    (next_nat >= heap_size ==>
+                      major' == update_all_objects_aux major (objects pos major) fwd 0) /\
+                    (next_nat + 8 < heap_size ==>
+                      Seq.mem (f_address (U64.uint_to_t next_nat)) (objects zero_addr major') /\
+                      Seq.length (objects (U64.uint_to_t next_nat) major') > 0)))
+
+val update_all_objects_positional_step_blue
+  (major: heap) (fwd: forwarding_map) (pos: hp_addr)
+  : Lemma (requires well_formed_heap_part1 major /\
+                    heap_objects_dense major /\
+                    U64.v pos + 8 < heap_size /\
+                    Seq.mem (f_address pos) (objects zero_addr major) /\
+                    Seq.length (objects pos major) > 0 /\
+                    is_blue (f_address pos) major)
+          (ensures (let hdr = read_word major pos in
+                    let wz = U64.v (getWosize hdr) in
+                    let obj : obj_addr = f_address pos in
+                    let next_nat = U64.v pos + (wz + 1) * 8 in
+                    next_nat <= heap_size /\ next_nat % 8 == 0 /\ next_nat < pow2 64 /\
+                    U64.v obj + wz * 8 <= heap_size /\
+                    (next_nat < heap_size ==>
+                      update_all_objects_aux major (objects (U64.uint_to_t next_nat) major) fwd 0 ==
+                        update_all_objects_aux major (objects pos major) fwd 0) /\
+                    (next_nat >= heap_size ==>
+                      major == update_all_objects_aux major (objects pos major) fwd 0) /\
+                    (next_nat + 8 < heap_size ==>
+                      Seq.mem (f_address (U64.uint_to_t next_nat)) (objects zero_addr major) /\
+                      Seq.length (objects (U64.uint_to_t next_nat) major) > 0)))
+
+val update_all_objects_terminal_step
+  (major: heap) (fwd: forwarding_map) (pos: hp_addr)
+  : Lemma (requires well_formed_heap_part1 major /\
+                    U64.v pos + 8 < heap_size /\
+                    Seq.mem (f_address pos) (objects zero_addr major) /\
+                    Seq.length (objects pos major) > 0 /\
+                    is_blue (f_address pos) major = false)
+          (ensures (let hdr = read_word major pos in
+                    let wz = U64.v (getWosize hdr) in
+                    let obj : obj_addr = f_address pos in
+                    let next_nat = U64.v pos + (wz + 1) * 8 in
+                    next_nat <= heap_size /\ next_nat % 8 == 0 /\
+                    U64.v obj + wz * 8 <= heap_size /\
+                    (next_nat + 8 >= heap_size ==>
+                      (let major' = update_object_pointers major obj wz fwd 0 in
+                       major' == update_all_objects_aux major (objects pos major) fwd 0))))
+
+val objects_initial_membership (g: heap)
+  : Lemma (requires heap_size > 8 /\ well_formed_heap_part1 g /\
+                    Seq.length (objects zero_addr g) > 0)
+          (ensures Seq.mem (f_address 0UL) (objects zero_addr g))
